$$
lost_k = 1 - \left( (1 - e^{-x+y\sqrt{1-P_{error_k}}t}) \times \frac{B(1-P_{error_k})}{G} \right)
$$

$$
P_{energy}\left(k\right)=1-e^{-\left\{x+y\left[1-P_{error}\left(k\right)\right]\right\}t}
$$

公式2
$$
P_{energy}\left(k\right)=1-e^{\frac{E(k,t=0)}{E(k,t)}t}
$$
3
$$
E\left(i,j\right)=B\mu+\eta\ BR^2
$$
4
$$
E\left(j,i\right)=B\mu
$$


5
$$
E\left(i\right)=2B\mu+\eta\ BR^2
$$
6
$$
P\left(i,i\in S\right)={\frac{1}{S}}
$$
7
$$
P\left(j->i\right)=\iint_{r}{P(i,i\in S)dS}=\frac{\pi r^2}{S}
$$
8
$$
P_{error}\left(i\right)=M\left(1-\frac{\pi r^2}{S}\right)
$$
9
$$
E\left(k,j\right)=B\mu+\eta\ BS\left[\frac{M-P_{error}\left(k\right)}{\pi M}\right]^2
$$
10
$$
P_{energy}\left(k\right)=1-e^{-\left\{x+y\left[1-P_{error}\left(k\right)\right]\right\}t}
$$
11
$$
x=\frac{2\mu}{E\left(k,t=0\right)}r
$$
12
$$
y=\frac{\eta\pi S}{NE\left(k,t=0\right)}r
$$



$$
E_{trans}[B,r]=E_{trans}\times E_{amp}\times r^{2}\times B
$$
